Exe/VeirOpt.lean
@@ -13,6 +13,7 @@ import Veir.Passes.InstructionSelection.RISCV64
 import Veir.Passes.InstructionSelection.RISCV64Sdag
 import Veir.Passes.InstructionSelection.RISCV64Branches
 import Veir.Passes.DCE.dce
+import Veir.Passes.SimplifyCFG
 import Veir.Passes.CastsReconciliation.Reconciliation
 import Veir.Passes.FunctionBoundaryCoercion.Coercion
 import Veir.Passes.RISCVCombines.Combine
@@ -41,6 +42,7 @@ def availablePasses : Std.HashMap String (Pass OpCode) :=
      IselSDAG,
      IselBrRISCV64,
      DCEPass,
+     SimplifyCFGPass,
      CastReconcilePass,
      CoerceFunctionBoundariesToRiscvRegPass,
      CoerceModArithFunctionBoundariesPass,
